Use FutureEtaExpand proof also in ArityEtaExpand proof

Launchbury/ArityEtaExpand.thy
@@ -1,26 +1,18 @@
 theory ArityEtaExpand
-imports ArityCorrectSestoft ArityEtaExpansionSestoft AbstractTransform
+imports ArityCorrectSestoft ArityEtaExpansionSestoft AbstractTransform ConstOn
 begin
 
-locale ArityEtaExpand = CorrectArityAnalysisLet
+locale CardinalityArityTransformation = CorrectArityAnalysisLetNoCard 
 begin
-  lemma Aeta_expand_pres_Aexp:
-  "Aexp (Aeta_expand n e)\<cdot>n = Aexp e\<cdot>n"
-    apply (induction n arbitrary:e rule: Arity_ind)
-    apply simp
-    apply (simp add: Aexp_App Aexp_Lam)
-    apply (subgoal_tac "fresh_var e \<notin> edom (Aexp e\<cdot>(inc\<cdot>n))")
-    apply simp
-    by (metis Aexp_lookup_fresh edomIff fresh_var_fresh)
 
   sublocale AbstractTransformBound
     "\<lambda> a . inc\<cdot>a"
     "\<lambda> a . pred\<cdot>a"
-    "\<lambda> \<Delta> e a . (a, Aheap \<Delta>\<cdot>(Aexp e\<cdot>a))"
-    "\<lambda> b . fst b"
-    "\<lambda> b . snd b"
+    "\<lambda> \<Delta> e a . (a, Aheap \<Delta> e\<cdot>a)"
+    "fst"
+    "snd"
     "Aeta_expand"
-    "\<lambda> b . snd b"
+    "snd"
   apply default
   apply (((rule eq_reflection)?, perm_simp, rule)+)[7]
   done
@@ -28,63 +20,26 @@ begin
   sublocale AbstractTransformBoundSubst
     "\<lambda> a . inc\<cdot>a"
     "\<lambda> a . pred\<cdot>a"
-    "\<lambda> \<Delta> e a . (a, Aheap \<Delta>\<cdot>(Aexp e\<cdot>a))"
-    "\<lambda> b . fst b"
-    "\<lambda> b . snd b"
+    "\<lambda> \<Delta> e a . (a, Aheap \<Delta> e\<cdot>a)"
+    "fst"
+    "snd"
     "Aeta_expand"
-    "\<lambda> b . snd b"
+    "snd"
   apply default
-  apply (simp add: Aheap_subst  Aheap_cong[OF Aexp_subst_restr])[1]
-  apply (rule subst_Aeta_expand)  
+  apply (simp add: Aheap_subst)
+  apply (rule subst_Aeta_expand)
   done
 
-  abbreviation Atransform where "Atransform \<equiv> transform"
-
- (*
-  lemma trans_pres_Aexp: "Aexp (Atransform a e)\<cdot>a = Aexp e\<cdot>a"
-  apply (nominal_induct e arbitrary: a  rule: exp_strong_induct)
-  apply (case_tac b)
-  apply simp_all[2]
-  apply (auto simp add: Aexp_App)[1]
-  defer
-  apply (auto cong add: Aexp_Lam)[1]
-  apply simp
-  apply (rule Aexp_Let_cong)
-  apply simp
-  defer
-  apply simp
-  thm Aheap_cong[where \<Gamma> = "map_transform Atransform (Aheap \<Gamma>\<cdot>(Aexp exp\<cdot>a)) \<Gamma>" and \<Gamma>' = \<Gamma> for \<Gamma> exp]
-  apply (subgoal_tac "Aheap (map_transform Atransform (Aheap \<Gamma>\<cdot>(Aexp exp\<cdot>a)) \<Gamma>)\<cdot>(Aexp exp\<cdot>a) = Aheap \<Gamma>\<cdot>(Aexp exp\<cdot>a)")
-  apply simp
-  defer
-  apply (rule Aheap_cong)
-    apply simp
-    apply (simp add: map_of_map_transform option.map_comp)
-  apply (rule Aheap_cong)
-    apply simp
-    apply (simp add: map_of_map_transform option.map_comp Aeta_expand_pres_Aexp)
-  done
-  
-  lemma trans_pres_Aheap: "Aheap (map_transform Atransform (Aheap \<Delta>\<cdot>ae) \<Delta>)\<cdot>ae = (Aheap \<Delta>\<cdot>ae)"
-    by (rule Aheap_cong) (simp_all add: map_of_map_transform trans_pres_Aexp)
-  *)
-
-  (* Check simp rules *)
-  lemma "transform a (App e x) = App (transform (inc\<cdot>a) e) x" by simp
-  lemma "transform a (Lam [x]. e) = Lam [x].(transform (pred\<cdot>a) e)" by simp
-  lemma "transform a (GVar b x) = GVar b x" by (cases b) simp_all
-  lemma "transform a (Terms.Let \<Delta> e) = Let (map_transform Aeta_expand (Aheap \<Delta>\<cdot>(Aexp e\<cdot>a)) (map_transform transform (Aheap \<Delta>\<cdot>(Aexp e\<cdot>a)) \<Delta>))
-           (transform a e)" by (simp del: Let_eq_iff)
+  abbreviation aTransform where "aTransform \<equiv> transform"
 
   lemma supp_transform: "supp (transform a e) \<subseteq> supp e"
     by (induction rule: transform.induct)
        (auto simp add: exp_assn.supp Let_supp dest!: set_mp[OF supp_map_transform] set_mp[OF supp_map_transform_step] )
   interpretation supp_bounded_transform transform
-    by default (auto simp add: fresh_def supp_transform)
-  
+    by default (auto simp add: fresh_def supp_transform) 
 
   fun conf_transform :: "(AEnv \<times> Arity) \<Rightarrow> conf \<Rightarrow> conf"
-  where "conf_transform (ae, a) (\<Gamma>, e, S) =
+  where "conf_transform (ae,  a) (\<Gamma>, e, S) =
     (map_transform Aeta_expand ae (map_transform transform ae \<Gamma>), 
      transform a e,
      S)"
@@ -92,229 +47,245 @@ begin
   inductive consistent :: "(AEnv \<times> Arity) \<Rightarrow> conf \<Rightarrow> bool" where
     consistentI[intro!]: 
     "edom ae \<subseteq> domA \<Gamma> \<union> upds S
-    \<Longrightarrow> upds S \<subseteq> edom ae
+    \<Longrightarrow> heap_upds_ok (\<Gamma>, S)
     \<Longrightarrow> Astack S \<sqsubseteq> a
-    \<Longrightarrow> Aexp e \<cdot> a \<sqsubseteq> ae
-    \<Longrightarrow> (\<And> x e. map_of \<Gamma> x = Some e \<Longrightarrow> Aexp' e \<cdot> (ae x) \<sqsubseteq> ae)
-    \<Longrightarrow> (\<And> x e. map_of \<Gamma> x = Some e \<Longrightarrow> \<not> isLam e \<Longrightarrow> ae x = up\<cdot>0)
-    \<Longrightarrow> ae ` ap S \<subseteq> {up\<cdot>0}
-    \<Longrightarrow> ae ` upds S \<subseteq> {up\<cdot>0}
+    \<Longrightarrow> ABinds \<Gamma>\<cdot>ae \<squnion> Aexp e\<cdot>a \<sqsubseteq> ae
+    \<Longrightarrow> const_on ae (thunks \<Gamma>) (up\<cdot>0)
+    \<Longrightarrow> const_on ae (ap S) (up\<cdot>0)
+    \<Longrightarrow> const_on ae (upds S) (up\<cdot>0)
     \<Longrightarrow> consistent (ae, a) (\<Gamma>, e, S)"  
   inductive_cases consistentE[elim!]: "consistent (ae, a) (\<Gamma>, e, S)"
-
-lemma foo:
-  fixes c c' R 
-  assumes "c \<Rightarrow>\<^sup>* c'" and "\<not> boring_step c'" and "consistent (ae,a) c"
-  shows "\<exists>ae' a'. consistent (ae',a') c' \<and> conf_transform (ae,a) c \<Rightarrow>\<^sup>* conf_transform (ae',a') c'"
-using assms
-proof(induction c c' arbitrary: ae a rule:step_induction)
-case (app\<^sub>1 \<Gamma> e x S)
-  from app\<^sub>1 have "consistent (ae, inc\<cdot>a) (\<Gamma>, e, Arg x # S)"  by (fastforce simp add: Aexp_App join_below_iff)
-  moreover
-  have "conf_transform (ae, a) (\<Gamma>, App e x, S) \<Rightarrow> conf_transform (ae, inc\<cdot>a) (\<Gamma>, e, Arg x # S)" by simp rule
-  ultimately
-  show ?case by (blast del: consistentI consistentE)
-next
+  
+  lemma foo:
+    fixes c c' R 
+    assumes "c \<Rightarrow>\<^sup>* c'" and "\<not> boring_step c'" and "consistent (ae,a) c"
+    shows "\<exists>ae' ce' a'. consistent (ae',a') c' \<and> conf_transform (ae,a) c \<Rightarrow>\<^sup>* conf_transform (ae',a') c'"
+  using assms
+  proof(induction c c' arbitrary: ae a rule:step_induction)
+  case (app\<^sub>1 \<Gamma> e x S)
+    from app\<^sub>1 have "consistent (ae, inc\<cdot>a) (\<Gamma>, e, Arg x # S)"
+      by (auto simp add: join_below_iff  dest!: below_trans[OF Aexp_App] elim: below_trans)
+    moreover
+    have "conf_transform (ae, a) (\<Gamma>, App e x, S) \<Rightarrow> conf_transform (ae, inc\<cdot>a) (\<Gamma>, e, Arg x # S)"
+      by simp rule
+    ultimately
+    show ?case by (blast del: consistentI consistentE)
+  next
 case (app\<^sub>2 \<Gamma> y e x S)
-  have "Aexp (e[y ::= x])\<cdot>(pred\<cdot>a) \<sqsubseteq> ae" using app\<^sub>2
-    apply (auto simp add:  join_below_iff)
-    apply (rule below_trans[OF monofun_cfun_fun[OF Aexp_subst_App_Lam]])
-    apply (auto simp add: Aexp_App Aexp_Lam join_below_iff)
-    done
-  hence "consistent (ae, pred \<cdot> a) (\<Gamma>, e[y::=x], S)"  using app\<^sub>2  by fastforce
+  {
+  have "Aexp (e[y::=x])\<cdot>(pred\<cdot>a) \<sqsubseteq> env_delete y ((Aexp e)\<cdot>(pred\<cdot>a)) \<squnion> AE_singleton x\<cdot>(up\<cdot>0)" by (rule Aexp_subst)
+  also have "env_delete y ((Aexp e)\<cdot>(pred\<cdot>a)) \<sqsubseteq> Aexp (Lam [y]. e)\<cdot>a" by (rule Aexp_Lam)
+  also have "\<dots> \<sqsubseteq> ae" using app\<^sub>2 by (auto simp add: join_below_iff)
+  also have "AE_singleton x\<cdot>(up\<cdot>0) \<sqsubseteq> ae" using app\<^sub>2 by auto
+  also have "ae \<squnion> ae = ae" by simp
+  finally  have "Aexp (e[y::=x])\<cdot>(pred\<cdot>a) \<sqsubseteq> ae" by this simp_all
+  }
+  then
+  have "consistent (ae, pred\<cdot>a) (\<Gamma>, e[y::=x], S)" using app\<^sub>2
+    by (auto elim: below_trans edom_mono  simp add: join_below_iff)
   moreover
   have "conf_transform (ae, a) (\<Gamma>, Lam [y]. e, Arg x # S) \<Rightarrow> conf_transform (ae, pred \<cdot> a) (\<Gamma>, e[y::=x], S)" by (simp add: subst_transform[symmetric]) rule
   ultimately
-  show ?case by (blast del: consistentI consistentE)
+  show ?case by (blast  del: consistentI consistentE)
 next
 case (thunk \<Gamma> x e S)
-  have "consistent (ae, 0) (delete x \<Gamma>, e, Upd x # S)" using thunk by (fastforce simp add: join_below_iff)
+  hence "x \<in> thunks \<Gamma>" by auto
+  hence [simp]: "x \<in> domA \<Gamma>" by (rule set_mp[OF thunks_domA])
+  hence "x \<notin> upds S" using thunk by (auto elim!: heap_upds_okE)
+
+  from thunk have "Aexp (Var x)\<cdot>a \<sqsubseteq> ae" by (auto simp add: join_below_iff)
+  from below_trans[OF Aexp_Var fun_belowD[OF this] ]
+  have "up\<cdot>a \<sqsubseteq> ae x".    
+  then obtain u where "ae x = up\<cdot>u" and "a \<sqsubseteq> u" by (cases "ae x") auto
+  hence [simp]: "x \<in> edom ae" by (simp add: edom_def)
+
+  have "ae x = up\<cdot>0" using thunk `x \<in> thunks \<Gamma>` by (auto)
+  hence "u = 0" using `ae x = up\<cdot>u` by simp
+
+  
+  from Abinds_reorder1[OF `map_of \<Gamma> x = Some e`] `ae x = up\<cdot>u`
+  have "ABinds (delete x \<Gamma>)\<cdot>ae \<squnion> Aexp e\<cdot>u = ABinds \<Gamma>\<cdot>ae" by (auto intro: join_comm)
+  also have "\<dots> \<sqsubseteq> ae" using thunk by (auto simp add: join_below_iff)
+  finally have "ABinds (delete x \<Gamma>)\<cdot>ae \<squnion> Aexp e\<cdot>u \<sqsubseteq> ae".
+  hence "consistent (ae, 0) (delete x \<Gamma>, e, Upd x # S)" using thunk `ae x = up\<cdot>u` `u = 0`
+    by (auto intro!: const_onI)
   moreover
-  {
-  from thunk
-  have "ae x = up\<cdot>0" by auto
-  with  `map_of \<Gamma> x = Some e`
-  have "map_of (map_transform Aeta_expand ae (map_transform Atransform ae \<Gamma>)) x = Some (transform 0 e)"
+
+  from  `map_of \<Gamma> x = Some e` `ae x = up\<cdot>0`
+  have "map_of (map_transform Aeta_expand ae (map_transform transform ae \<Gamma>)) x = Some (transform 0 e)"
     by (simp add: map_of_map_transform)
   with `\<not> isLam e`
   have "conf_transform (ae, a) (\<Gamma>, Var x, S) \<Rightarrow> conf_transform (ae, 0) (delete x \<Gamma>, e, Upd x # S)"
-    by (auto simp add: map_transform_delete intro!: step.intros)
-  }
+    by (auto simp add: map_transform_delete restr_delete_twist intro!: step.intros  simp del: restr_delete)
   ultimately
   show ?case by (blast del: consistentI consistentE)
 next
 case (lamvar \<Gamma> x e S)
-  from lamvar have "ae ` upds S \<subseteq> {up \<cdot> 0}" by fastforce
-  from lamvar have "Astack S \<sqsubseteq> a" by auto
-
-  from lamvar have "Aexp (Var x)\<cdot>a \<sqsubseteq> ae" by auto
+  from lamvar have [simp]: "x \<in> domA \<Gamma>" by auto (metis domI dom_map_of_conv_domA)
+  from lamvar have "Aexp (Var x)\<cdot>a \<sqsubseteq> ae" by (auto simp add: join_below_iff)
   from below_trans[OF Aexp_Var fun_belowD[OF this] ]
   have "up\<cdot>a \<sqsubseteq> ae x".
   then obtain u where "ae x = up\<cdot>u" and "a \<sqsubseteq> u" by (cases "ae x") auto
 
-  have "Aexp' e\<cdot>(ae x) \<sqsubseteq> ae" using lamvar by auto
-  hence "Aexp e\<cdot>u \<sqsubseteq> ae" using `ae x = up\<cdot>u` by simp
-  then
+  from Abinds_reorder1[OF `map_of \<Gamma> x = Some e`] `ae x = up\<cdot>u`
+  have "ABinds (delete x \<Gamma>)\<cdot>ae \<squnion> Aexp e\<cdot>u = ABinds \<Gamma>\<cdot>ae" by (auto intro: join_comm)
+  also have "\<dots> \<sqsubseteq> ae" using lamvar by (auto simp add: join_below_iff)
+  finally have "ABinds (delete x \<Gamma>)\<cdot>ae \<squnion> Aexp e\<cdot>u \<sqsubseteq> ae".
+
   have "consistent (ae, u) ((x, e) # delete x \<Gamma>, e, S)"
-    using lamvar by (auto  simp add: join_below_iff split:if_splits intro: below_trans[OF _ `a \<sqsubseteq> u`])
+    using lamvar `ABinds (delete x \<Gamma>)\<cdot>ae \<squnion> Aexp e\<cdot>u \<sqsubseteq> ae`  `ae x = up\<cdot>u` 
+    by (auto simp add: join_below_iff split:if_splits intro: below_trans[OF _ `a \<sqsubseteq> u`] intro!: const_onI)
   moreover
+
+  have "Astack S \<sqsubseteq> u" using lamvar  below_trans[OF _ `a \<sqsubseteq> u`] by auto
+
   {
   from `isLam e`
-  have "isLam (Atransform u e)" by simp
-  hence "isLam (Aeta_expand u (Atransform u e))" by (rule isLam_Aeta_expand)
+  have "isLam (transform u e)" by simp
+  hence "isLam (Aeta_expand u (transform u e))" by (rule isLam_Aeta_expand)
   moreover
-  from  `map_of \<Gamma> x = Some e`  `ae x = up \<cdot> u`
-  have "map_of (map_transform Aeta_expand ae (map_transform Atransform ae \<Gamma>)) x = Some (Aeta_expand u (Atransform u e))"
+  from  `map_of \<Gamma> x = Some e`  `ae x = up \<cdot> u`  `isLam (transform u e)`
+  have "map_of (map_transform Aeta_expand ae (map_transform transform ae \<Gamma>)) x = Some (Aeta_expand u (transform u e))"
     by (simp add: map_of_map_transform)
   ultimately
   have "conf_transform (ae, a) (\<Gamma>, Var x, S) \<Rightarrow>\<^sup>*
-        ((x, Aeta_expand u (Atransform u e)) # (map_transform Aeta_expand ae (map_transform Atransform ae (delete x \<Gamma>))), Aeta_expand u  (Atransform u e), S)"
-     by (auto intro: lambda_var simp add: map_transform_delete)
-  also have "\<dots> = ((map_transform Aeta_expand ae (map_transform Atransform ae ((x,e) # delete x \<Gamma>))), Aeta_expand u  (Atransform u e), S)"
-    using `ae x = up \<cdot> u` by (simp add: map_transform_Cons)
+        ((x, Aeta_expand u (transform u e)) # delete x (map_transform Aeta_expand ae (map_transform transform ae \<Gamma>)), Aeta_expand u  (transform u e), S)"
+     by (auto intro: lambda_var simp add: map_transform_delete simp del: restr_delete)
+  also have "\<dots> = ((map_transform Aeta_expand ae (map_transform transform ae ((x,e) # delete x \<Gamma>))), Aeta_expand u (transform u e), S)"
+    using `ae x = up \<cdot> u` `isLam (transform u e)`
+    by (simp add: map_transform_Cons map_transform_delete restr_delete_twist del: restr_delete)
   also(subst[rotated]) have "\<dots> \<Rightarrow>\<^sup>* conf_transform (ae, u) ((x, e) # delete x \<Gamma>, e, S)"
-    by simp (rule Aeta_expand_correct[OF below_trans[OF `Astack S \<sqsubseteq> a` `a \<sqsubseteq> u`]])
+    by simp (rule Aeta_expand_correct[OF `Astack S \<sqsubseteq> u`])
   finally(rtranclp_trans)
   have "conf_transform (ae, a) (\<Gamma>, Var x, S) \<Rightarrow>\<^sup>* conf_transform (ae, u) ((x, e) # delete x \<Gamma>, e, S)".
   }
   ultimately show ?case by (blast del: consistentI consistentE)
 next
 case (var\<^sub>2 \<Gamma> x e S)
-  hence "ae x = up\<cdot>0" by auto
+
+  have "ae x = up\<cdot>a" using var\<^sub>2 by auto
 
   have "Astack (Upd x # S) \<sqsubseteq> a" using var\<^sub>2 by auto
   hence "a = 0" by auto
 
   have "consistent (ae, 0) ((x, e) # \<Gamma>, e, S)" using var\<^sub>2
-    by (fastforce  simp add: join_below_iff split:if_splits)
+    by (auto simp add: join_below_iff split:if_splits)
   moreover
   have "conf_transform (ae, a) (\<Gamma>, e, Upd x # S) \<Rightarrow> conf_transform (ae, 0) ((x, e) # \<Gamma>, e, S)"
-    using `ae x = up\<cdot>0` `a = 0` var\<^sub>2 by (auto intro!: step.intros simp add: map_transform_Cons)
+    using `ae x = up\<cdot>a` `a = 0` var\<^sub>2
+    by (auto intro!: step.intros simp add: map_transform_Cons)
   ultimately show ?case by (blast del: consistentI consistentE)
 next
   case (let\<^sub>1 \<Delta> \<Gamma> e S)
 
-  let ?ae = "Aheap \<Delta> \<cdot> (Aexp e\<cdot>a)"
+  let ?ae = "Aheap \<Delta> e\<cdot>a"
   let ?new = "(domA (\<Delta> @ \<Gamma>) \<union> upds S - (domA \<Gamma> \<union> upds S))"
   have new: "?new = domA \<Delta>"
     using fresh_distinct[OF let\<^sub>1(1)] fresh_distinct_fv[OF let\<^sub>1(2)]
     by (auto dest: set_mp[OF ups_fv_subset])
 
   have "domA \<Delta> \<inter> upds S = {}" using fresh_distinct_fv[OF let\<^sub>1(2)] by (auto dest: set_mp[OF ups_fv_subset])
-  hence *: "\<And> x. x \<in> upds S \<Longrightarrow> x \<notin> edom (Aheap \<Delta>\<cdot>(Aexp e\<cdot>a))"
-    using edom_Aheap[where \<Gamma> = \<Delta> and ae = "Aexp e\<cdot>a"] by auto
+  hence *: "\<And> x. x \<in> upds S \<Longrightarrow> x \<notin> edom ?ae" by (auto dest!: set_mp[OF edom_Aheap])
 
-  have "edom ae \<subseteq> - domA \<Delta>" using let\<^sub>1(3)
-    using fresh_distinct[OF let\<^sub>1(1)] fresh_distinct_fv[OF let\<^sub>1(2)]
-    by (fastforce dest: set_mp[OF ups_fv_subset])
-  hence "(?ae \<squnion> ae) f|` (- domA \<Delta>) = ae"
-    by (auto simp add: env_restr_join  env_restr_useless disjoint_eq_subset_Compl edom_Aheap)
-  moreover
+  have restr_stack_simp: "restr_stack (edom (?ae \<squnion> ae)) S = restr_stack (edom ae) S"
+    by (auto intro: restr_stack_cong dest!: *)
+
+  have "edom ae \<subseteq> domA \<Gamma> \<union> upds S" using let\<^sub>1 by auto
+  from set_mp[OF this] fresh_distinct[OF let\<^sub>1(1)] fresh_distinct_fv[OF let\<^sub>1(2)]
+  have [simp]: "ae f|` domA \<Delta> = \<bottom>"
+    using  fresh_distinct[OF let\<^sub>1(1)] by (auto dest: set_mp[OF ups_fv_subset])
+
+  from  fresh_distinct[OF let\<^sub>1(1)]
+   have [simp]: "?ae f|` domA \<Gamma> = \<bottom>" by (auto dest!: set_mp[OF edom_Aheap])
+
   {
   have "edom (?ae \<squnion> ae) \<subseteq> domA (\<Delta> @ \<Gamma>) \<union> upds S"
     using let\<^sub>1(3) by (auto dest: set_mp[OF edom_Aheap])
   moreover
-  have "upds S \<subseteq> edom (?ae \<squnion> ae)"
-    using let\<^sub>1(3) by auto
+  have "const_on (?ae \<squnion> ae) (thunks \<Gamma>) (up\<cdot>0)" using let\<^sub>1 by fastforce
   moreover
   { fix x e'
-    assume "map_of \<Delta> x = Some e'"
-    hence "x \<notin> edom ae" using `edom ae \<subseteq> - domA \<Delta>` by (metis Compl_iff contra_subsetD domI dom_map_of_conv_domA)
-    hence "Aexp' e'\<cdot>((?ae \<squnion> ae) x) = Aexp' e'\<cdot>(?ae x)" by (auto simp add: edomIff)
-    also
-    have "Aexp' e'\<cdot>(?ae x) \<sqsubseteq> (Aexp' e'\<cdot>(?ae x) f|` domA \<Delta>) \<squnion> (Aexp' e'\<cdot>(?ae x) f|` (- domA \<Delta>))"
-      by (rule eq_imp_below[OF join_env_restr_UNIV[symmetric]]) auto
-    also
-    from `map_of \<Delta> x = Some e'`
-    have "Aexp' e'\<cdot>(?ae x) f|` domA \<Delta> \<sqsubseteq> ?ae" by (rule Aheap_heap)
-    also
-    from `map_of \<Delta> x = Some e'`
-    find_theorems Aheap name:heap
-    have "Aexp' e'\<cdot>(?ae x) f|` (- domA \<Delta>) \<sqsubseteq> Aexp (Terms.Let \<Delta> e)\<cdot>a" by (rule Aheap_heap2)
-    also
-    have "Aexp (Terms.Let \<Delta> e)\<cdot>a \<sqsubseteq> ae" using let\<^sub>1(3) by auto
-    finally
-    have "Aexp' e'\<cdot>((?ae \<squnion> ae) x) \<sqsubseteq> ?ae \<squnion> ae" by this auto
+    assume "x \<in> thunks \<Delta>" 
+    hence "x \<notin> domA \<Gamma>" and "x \<notin> upds S"
+      using fresh_distinct[OF let\<^sub>1(1)] fresh_distinct_fv[OF let\<^sub>1(2)]
+      by (auto dest!: set_mp[OF thunks_domA] set_mp[OF ups_fv_subset])
+    hence "(?ae \<squnion> ae) x = up \<cdot> 0" using `x \<in> thunks \<Delta>` by (auto simp add: Aheap_heap3)
   }
+  hence "const_on (?ae \<squnion> ae) (thunks \<Delta>) (up\<cdot>0)" by auto
   moreover
-  { fix x e'
-    assume "map_of \<Gamma> x = Some e'"
-    hence "x \<in> domA \<Gamma>" by (metis domI dom_map_of_conv_domA)
-    hence "x \<notin> edom ?ae" using fresh_distinct[OF let\<^sub>1(1)]  by (auto dest: set_mp[OF edom_Aheap])
-    with let\<^sub>1 `map_of \<Gamma> x = Some e'`
-    have "Aexp' e'\<cdot>((?ae \<squnion> ae) x) \<sqsubseteq> ae" by (auto simp add: edomIff)
-    hence "Aexp' e'\<cdot>((?ae \<squnion> ae) x) \<sqsubseteq> ?ae \<squnion> ae" by (metis (erased, hide_lams) "HOLCF-Join-Classes.join_above2" below_trans)
-  }
+  have "const_on ae (ap S) (up\<cdot>0)" using let\<^sub>1 by auto  
+  hence "const_on (?ae \<squnion> ae) (ap S) (up\<cdot>0)" by fastforce
   moreover
-  { fix x e'
-    assume "\<not> isLam e'"
-    assume "map_of \<Gamma> x = Some e'"
-    hence "x \<in> domA \<Gamma>" by (metis domI dom_map_of_conv_domA)
-    hence "x \<notin> edom ?ae" using fresh_distinct[OF let\<^sub>1(1)]  by (auto dest: set_mp[OF edom_Aheap])
-    with let\<^sub>1 `map_of \<Gamma> x = Some e'` `\<not> isLam e'`
-    have "(?ae \<squnion> ae) x = up \<cdot>0" by (auto simp add: edomIff)
-  }
+  have "const_on ae (upds S) (up\<cdot>0)" using let\<^sub>1 by auto
+  hence "const_on (?ae \<squnion> ae) (upds S) (up\<cdot>0)"  by fastforce
   moreover
-  { fix x e'
-    assume "map_of \<Delta> x = Some e'" and "\<not> isLam e'"
-    hence "?ae x = up \<cdot> 0" using Aheap_heap3 by auto
-    hence "(?ae \<squnion> ae) x = up \<cdot> 0" by simp
-  }
+  have "Astack S \<sqsubseteq> a" unfolding restr_stack_simp using let\<^sub>1 by auto
   moreover
-  have "(?ae \<squnion> ae) ` upds S \<subseteq> {up \<cdot> 0}" using let\<^sub>1 * by fastforce
-  moreover
-  have "(?ae \<squnion> ae) ` ap S \<subseteq> {up \<cdot> 0}" using let\<^sub>1 * by fastforce
-  moreover
-  have "Astack S \<sqsubseteq> a"  using let\<^sub>1 by auto
+  have "heap_upds_ok (\<Gamma>, S)" using let\<^sub>1 by auto
+  with fresh_distinct[OF let\<^sub>1(1)]  `domA \<Delta> \<inter> upds S = {}`
+  have "heap_upds_ok (\<Delta> @ \<Gamma>, S)" by (rule heap_upds_ok_append)
   moreover
   {
-  have "Aexp e\<cdot>a \<sqsubseteq> (Aexp e\<cdot>a f|` domA \<Delta>) \<squnion> (Aexp e\<cdot>a f|` (- domA \<Delta>))"
-    by (rule eq_imp_below[OF join_env_restr_UNIV[symmetric]]) auto
-  also have "Aexp e\<cdot>a f|` (- domA \<Delta>) \<sqsubseteq> Aexp (Terms.Let \<Delta> e)\<cdot>a" by (rule Aexp_Let_above)
-  also have "\<dots> \<sqsubseteq> ae" using let\<^sub>1(3) by auto
-  also have "Aexp e\<cdot>a f|` domA \<Delta> \<sqsubseteq> ?ae" by (rule Aheap_above_arg)
-  finally have "Aexp e\<cdot>a \<sqsubseteq> ?ae \<squnion> ae" by this auto
+  have "ABinds \<Delta>\<cdot>(Aheap \<Delta> e\<cdot>a \<squnion> ae) = ABinds \<Delta>\<cdot>(Aheap \<Delta> e\<cdot>a)"
+    by (rule Abinds_env_restr_cong) (simp add: env_restr_join)
+  moreover
+  have "ABinds \<Gamma>\<cdot>(Aheap \<Delta> e\<cdot>a \<squnion> ae) = ABinds \<Gamma>\<cdot>ae"
+    by (rule Abinds_env_restr_cong) (simp add: env_restr_join)
+  ultimately
+  have "ABinds (\<Delta> @ \<Gamma>) \<cdot> (Aheap \<Delta> e\<cdot>a \<squnion> ae) \<squnion> Aexp e\<cdot>a = (ABinds \<Delta>\<cdot>(Aheap \<Delta> e\<cdot>a) \<squnion> Aexp e\<cdot>a) \<squnion> ABinds \<Gamma>\<cdot>ae"
+    apply (simp add: Abinds_append_disjoint[OF fresh_distinct[OF let\<^sub>1(1)]])
+    by (metis join_comm)
+  moreover have "(ABinds \<Delta>\<cdot>(Aheap \<Delta> e\<cdot>a) \<squnion> Aexp e\<cdot>a) \<sqsubseteq> Aheap \<Delta> e\<cdot>a \<squnion> Aexp (Let \<Delta> e)\<cdot>a" by (rule Aexp_Let)
+  moreover have " ABinds \<Gamma>\<cdot>ae \<squnion> Aexp (Let \<Delta> e)\<cdot>a \<sqsubseteq> ae" using let\<^sub>1 by auto
+  ultimately
+  have "ABinds (\<Delta> @ \<Gamma>) \<cdot> (Aheap \<Delta> e\<cdot>a \<squnion> ae) \<squnion> Aexp e\<cdot>a \<sqsubseteq> Aheap \<Delta> e\<cdot>a \<squnion> ae"
+    apply (simp only: join_assoc[symmetric])
+    apply (erule below_trans[OF join_mono[OF _ below_refl]])
+    apply (simp only: join_assoc)
+    apply (subst join_comm) back
+    apply (erule join_mono[OF  below_refl])
+    done
   }
   ultimately
-  have "consistent (?ae \<squnion> ae, a) (\<Delta> @ \<Gamma>, e, S) "
-    by auto
+  have "consistent (?ae \<squnion> ae, a) (\<Delta> @ \<Gamma>, e, S) " by auto
   }
   moreover
   {
-    have "\<And> x. x \<in> domA \<Gamma> \<Longrightarrow> x \<notin> edom (Aheap \<Delta>\<cdot>(Aexp e\<cdot>a))"
+    have "\<And> x. x \<in> domA \<Gamma> \<Longrightarrow> x \<notin> edom ?ae"
       using fresh_distinct[OF let\<^sub>1(1)]
       by (auto dest!: set_mp[OF edom_Aheap])
-    hence "map_transform Aeta_expand ((Aheap \<Delta>\<cdot>(Aexp e\<cdot>a)) \<squnion> ae) (map_transform Atransform ((Aheap \<Delta>\<cdot>(Aexp e\<cdot>a)) \<squnion> ae) \<Gamma>)
-       = map_transform Aeta_expand ae (map_transform Atransform ae \<Gamma>)"
-      by (auto intro!: map_transform_cong simp add: edomIff)
+    hence "map_transform Aeta_expand (?ae \<squnion> ae) (map_transform transform (?ae \<squnion> ae) \<Gamma>)
+       = map_transform Aeta_expand ae (map_transform transform ae \<Gamma>)"
+       by (auto intro!: map_transform_cong restrictA_cong simp add: edomIff)
     moreover
+
     from let\<^sub>1 have *: "edom ae \<subseteq> domA \<Gamma> \<union> upds S" by auto
     have "\<And> x. x \<in> domA \<Delta> \<Longrightarrow> x \<notin> edom ae"
        using fresh_distinct[OF let\<^sub>1(1)] fresh_distinct_fv[OF let\<^sub>1(2)] 
        by (auto dest!: set_mp[OF *] set_mp[OF ups_fv_subset])
-    hence "map_transform Aeta_expand ((Aheap \<Delta>\<cdot>(Aexp e\<cdot>a)) \<squnion> ae) (map_transform Atransform ((Aheap \<Delta>\<cdot>(Aexp e\<cdot>a)) \<squnion> ae) \<Delta>)
-       = map_transform Aeta_expand ((Aheap \<Delta>\<cdot>(Aexp e\<cdot>a))) (map_transform Atransform ((Aheap \<Delta>\<cdot>(Aexp e\<cdot>a))) \<Delta>)"
-      by (auto intro!: map_transform_cong simp add: edomIff)
+    hence "map_transform Aeta_expand (?ae \<squnion> ae) (map_transform transform (?ae \<squnion> ae) \<Delta>)
+       = map_transform Aeta_expand ?ae (map_transform transform ?ae \<Delta>)"
+       by (auto intro!: map_transform_cong restrictA_cong simp add: edomIff)
     ultimately
-    have "conf_transform (ae, a) (\<Gamma>, Terms.Let \<Delta> e, S) \<Rightarrow> conf_transform (?ae \<squnion> ae, a) (\<Delta> @ \<Gamma>, e, S)"
-      apply (simp add: map_transform_append)
-      apply rule
-      using let\<^sub>1(1,2)
-      by auto
+
+    have "conf_transform (ae, a) (\<Gamma>, Let \<Delta> e, S) \<Rightarrow> conf_transform (?ae \<squnion> ae, a) (\<Delta> @ \<Gamma>, e, S)"
+      using  let\<^sub>1(1,2)
+      by (fastforce intro!: step.intros simp add: map_transform_append  dest: set_mp[OF edom_Aheap])
   }
   ultimately
-  show ?case  by (blast del: consistentI consistentE)
+  show ?case by (blast del: consistentI consistentE)
 next
   case refl thus ?case by auto
 next
-  case trans
-    from trans(5)
-    show ?case
-      apply (auto dest!: trans(3,4))
-      apply (metis (poly_guards_query) rtranclp_trans)
-      done
+  case (trans c c' c'')
+    from trans(3)[OF trans(5)]
+    obtain ae' a' where "consistent (ae', a') c'" and *: "conf_transform (ae, a) c \<Rightarrow>\<^sup>* conf_transform (ae', a') c'" by blast
+    from trans(4)[OF this(1)]
+    obtain ae'' a'' where "consistent (ae'', a'') c''" and **: "conf_transform (ae', a') c' \<Rightarrow>\<^sup>* conf_transform (ae'', a'') c''" by blast
+    from this(1) rtranclp_trans[OF * **]
+    show ?case by blast
 qed
 
 end
-end
 
+end
